src/theory/bir/bir_typing_expSyntax.sig
@@ -12,11 +12,6 @@ sig
    val is_bir_vars_of_exp   : term -> bool
    val mk_bir_vars_of_exp   : term -> term
 
-   val bir_var_set_is_well_typed_tm   : term
-   val dest_bir_var_set_is_well_typed : term -> term
-   val is_bir_var_set_is_well_typed   : term -> bool
-   val mk_bir_var_set_is_well_typed   : term -> term
-
    val bir_exp_is_well_typed_tm   : term
    val dest_bir_exp_is_well_typed : term -> term
    val is_bir_exp_is_well_typed   : term -> bool
