src/theory/bir/bir_envScript.sml
@@ -23,11 +23,18 @@ SIMP_TAC std_ss [bir_var_type_def, bir_var_name_def, bir_var_t_11])
 val _ = Datatype `bir_var_environment_t = BEnv (string -> (bir_val_t option))`;
 val bir_var_environment_t_11 = DB.fetch "-" "bir_var_environment_t_11";
 
+(* Empty environment *)
+val bir_empty_env_def = Define `bir_empty_env = BEnv (K NONE)`
+
 val bir_env_lookup_def = Define `
   (bir_env_lookup varname (BEnv env) = env varname)`;
 
 val bir_env_update_def = Define `
-  (bir_env_update varname v (BEnv env) = BEnv ((varname =+ SOME v) env))`;
+    bir_env_update varname v ty (BEnv env) =
+      if (ty = (type_of_bir_val v)) /\ (env varname <> NONE) then
+        SOME (BEnv ((varname =+ SOME v) env))
+      else
+        NONE`;
 
 val bir_env_lookup_UPDATE = store_thm ("bir_env_lookup_UPDATE",
 ``bir_env_lookup vn (BEnv ((vn' =+ vo) env)) =
@@ -64,8 +71,8 @@ SIMP_TAC std_ss [bir_env_read_def, bir_env_lookup_UPDATE,
 Cases_on `bir_var_name var = vn` >> ASM_SIMP_TAC std_ss []);
 
 val bir_env_write_def = Define `bir_env_write var va env =
-	 if (bir_env_check_type var env) /\ ((bir_var_type var) = (type_of_bir_val va)) then
-	   SOME (bir_env_update (bir_var_name var) va env)
+	 if (bir_env_check_type var env) then
+	   bir_env_update (bir_var_name var) va (bir_var_type var) env
 	 else
 	   NONE
 `;
@@ -85,8 +92,8 @@ val bir_env_write_types = store_thm ("bir_env_write_types",
     (bir_env_write v va env = SOME env') ==>
     (bir_env_lookup_type (bir_var_name v) env = bir_env_lookup_type (bir_var_name v) env')``,
 
-SIMP_TAC std_ss [bir_env_write_def, bir_env_check_type_def] >>
 Cases_on `env` >>
+SIMP_TAC std_ss [bir_env_write_def, bir_env_update_def, bir_env_check_type_def] >>
 REWRITE_TAC [bir_env_update_def, bir_env_lookup_type_def, bir_env_lookup_type_def, bir_env_lookup_UPDATE] >>
 SIMP_TAC std_ss []
 );
@@ -132,6 +139,14 @@ val bir_env_satisfies_envty_of_env = store_thm("bir_env_satisfies_envty_of_env",
   SIMP_TAC std_ss [bir_env_satisfies_envty_def, bir_envty_of_env_def] >>
   METIS_TAC[]
 );
+
+(*
+TODO: typing is preserved by write
+"bir_env_update_is_well_typed_env"
+(bir_is_well_typed_env env /\
+    (bir_env_update varname vo ty env = SOME env')) ==>
+    bir_is_well_typed_env env'
+*)
 
 val bir_envty_includes_v_def = Define `bir_envty_includes_v (BEnvTy envty) v =
   (envty (bir_var_name v) = SOME (bir_var_type v))
@@ -217,186 +232,6 @@ val bir_envty_includes_vs_SUBSET = store_thm("bir_envty_includes_vs_SUBSET", ``
   SIMP_TAC std_ss [bir_envty_includes_vs_def, SUBSET_DEF] >>
   METIS_TAC[]
 );
-
-
-
-
-
-(* ===================== *)
-(*
-bir_vs_consistent!!!
-
-val bir_var_set_is_well_typed_def = Define `bir_var_set_is_well_typed vs <=>
-  (!v1 v2. (v1 IN vs /\ v2 IN vs /\ (bir_var_name v1 = bir_var_name v2)) ==>
-           (bir_var_type v1 = bir_var_type v2))`;
-
-val bir_var_set_is_well_typed_INJ_DEF = store_thm ("bir_var_set_is_well_typed_INJ_DEF",
-  ``bir_var_set_is_well_typed vs <=> INJ bir_var_name vs UNIV``,
-
-SIMP_TAC std_ss [bir_var_set_is_well_typed_def, INJ_DEF, IN_UNIV,
-  bir_var_eq_EXPAND] >>
-METIS_TAC[]);
-
-val bir_var_set_is_well_typed_EMPTY = store_thm ("bir_var_set_is_well_typed_EMPTY",
-  ``bir_var_set_is_well_typed {}``,
-SIMP_TAC std_ss [bir_var_set_is_well_typed_def, NOT_IN_EMPTY]);
-
-val bir_var_set_is_well_typed_INSERT = store_thm ("bir_var_set_is_well_typed_INSERT",
-  ``!v vs. bir_var_set_is_well_typed (v INSERT vs) <=>
-           bir_var_set_is_well_typed vs /\
-           (!v'. v' IN vs ==>
-                 (bir_var_name v = bir_var_name v') ==>
-                 (bir_var_type v = bir_var_type v'))``,
-
-SIMP_TAC std_ss [bir_var_set_is_well_typed_def, IN_INSERT] >>
-METIS_TAC[]);
-
-
-val bir_var_set_is_well_typed_UNION = store_thm ("bir_var_set_is_well_typed_UNION",
-``!vs1 vs2. bir_var_set_is_well_typed (vs1 UNION vs2) <=>
-            bir_var_set_is_well_typed vs1 /\
-            bir_var_set_is_well_typed vs2 /\
-            (!v1 v2. v1 IN vs1 ==> v2 IN vs2 ==>
-                 (bir_var_name v1 = bir_var_name v2) ==>
-                 (bir_var_type v1 = bir_var_type v2))``,
-
-SIMP_TAC std_ss [bir_var_set_is_well_typed_def, IN_UNION] >>
-METIS_TAC[]);
-
-
-val bir_var_set_is_well_typed_SUBSET = store_thm ("bir_var_set_is_well_typed_SUBSET",
-  ``!vs1 vs2. vs1 SUBSET vs2 ==> bir_var_set_is_well_typed vs2 ==> bir_var_set_is_well_typed vs1``,
-SIMP_TAC std_ss [bir_var_set_is_well_typed_def, SUBSET_DEF] >>
-METIS_TAC[]);
-
-
-val bir_env_vars_are_initialised_WELL_TYPED = store_thm ("bir_env_vars_are_initialised_WELL_TYPED",
-  ``!vs env. bir_env_vars_are_initialised env vs ==> bir_var_set_is_well_typed vs``,
-
-  SIMP_TAC std_ss [bir_var_set_is_well_typed_def, bir_env_vars_are_initialised_def] >>
-  REPEAT STRIP_TAC >>
-  Cases_on `v1` >> Cases_on `v2` >>
-  rename1 `bir_var_name (BVar vn1 vty1) = bir_var_name (BVar vn2 vty2)` >>
-  FULL_SIMP_TAC std_ss [bir_var_name_def, bir_var_type_def] >>
-
-
-  `bir_env_var_is_initialised env (BVar vn2 vty1)` by METIS_TAC[] >>
-  `bir_env_var_is_initialised env (BVar vn2 vty2)` by METIS_TAC[] >>
-  FULL_SIMP_TAC std_ss [bir_env_var_is_initialised_def, bir_var_type_def, bir_var_name_def] >>
-  FULL_SIMP_TAC std_ss []
-);
-
-
-val bir_env_vars_are_initialised_SUBSET_DOMAIN = store_thm ("bir_env_vars_are_initialised_SUBSET_DOMAIN",
-  ``!vs env. bir_env_vars_are_initialised env vs ==>
-             (IMAGE bir_var_name vs) SUBSET (bir_env_domain env)``,
-
-REPEAT STRIP_TAC >>
-Cases_on `env` >> rename1 `BEnv env` >>
-FULL_SIMP_TAC std_ss [bir_env_vars_are_initialised_def, SUBSET_DEF, IN_IMAGE,
-  PULL_EXISTS, bir_env_domain_def] >>
-REPEAT STRIP_TAC >>
-rename1 `v IN vs` >>
-Q.PAT_X_ASSUM `!v. _` (MP_TAC o Q.SPEC `v`) >>
-Cases_on `v` >> rename1 `BVar vn vty` >>
-ASM_SIMP_TAC std_ss [bir_env_var_is_initialised_def, bir_env_lookup_def,
-    flookup_thm, PULL_EXISTS, bir_var_name_def]);
-
-
-val VAR_SET_FINITE_IFF_NAME_SET_FINITE = store_thm ("VAR_SET_FINITE_IFF_NAME_SET_FINITE",
-``!vs. FINITE vs <=> FINITE (IMAGE bir_var_name vs)``,
-
-GEN_TAC >> EQ_TAC >- (
-  METIS_TAC[IMAGE_FINITE]
-) >>
-STRIP_TAC >>
-Q.ABBREV_TAC `VS = BIGUNION (IMAGE (\vn. IMAGE (\ty. BVar vn ty) UNIV) (IMAGE bir_var_name vs))` >>
-`vs SUBSET VS` by (
-  Q.UNABBREV_TAC `VS` >>
-  SIMP_TAC std_ss [SUBSET_DEF, IN_BIGUNION, IN_IMAGE, PULL_EXISTS, IN_UNIV] >>
-  REPEAT STRIP_TAC >>
-  rename1 `v IN vs` >>
-  Q.EXISTS_TAC `v` >>
-  Q.EXISTS_TAC `bir_var_type v` >>
-  Cases_on `v` >>
-  ASM_SIMP_TAC std_ss [bir_var_type_def, bir_var_name_def]
-) >>
-
-`FINITE VS` suffices_by METIS_TAC[SUBSET_FINITE] >>
-Q.UNABBREV_TAC `VS` >>
-SIMP_TAC std_ss [FINITE_BIGUNION_EQ, IN_IMAGE, PULL_EXISTS] >>
-METIS_TAC[IMAGE_FINITE, bir_type_t_FINITE_UNIV]);
-
-
-val bir_env_vars_are_initialised_FINITE = store_thm ("bir_env_vars_are_initialised_FINITE",
-  ``!vs env. bir_env_vars_are_initialised env vs ==> FINITE vs``,
-
-METIS_TAC[bir_env_vars_are_initialised_SUBSET_DOMAIN, bir_env_domain_FINITE,
-          VAR_SET_FINITE_IFF_NAME_SET_FINITE, SUBSET_FINITE]);
-
-
-
-val bir_env_vars_are_initialised_ENV_EXISTS_EXTENSION = store_thm ("bir_env_vars_are_initialised_ENV_EXISTS_EXTENSION",
-  ``!vs1 vs2 env1.
-      (FINITE vs2 /\ vs1 SUBSET vs2 /\ bir_var_set_is_well_typed vs2) ==>
-      bir_env_vars_are_initialised env1 vs1 ==>
-      (?env2. bir_env_EQ_FOR_VARS vs1 env1 env2 /\
-              bir_env_vars_are_initialised env2 vs2)``,
-
-REPEAT STRIP_TAC >>
-Cases_on `env1` >> rename1 `BEnv env` >>
-Q.ABBREV_TAC `VF = (\v. (bir_var_type v, SOME (bir_default_value_of_type (bir_var_type v))))` >>
-Q.ABBREV_TAC `M1 = FUN_FMAP VF (vs2 DIFF vs1)` >>
-EXISTS_TAC ``BEnv (FUNION (MAP_KEYS bir_var_name M1) env)`` >>
-
-`FDOM M1 = vs2 DIFF vs1` by METIS_TAC[FDOM_FMAP, FINITE_DIFF] >>
-`INJ bir_var_name (FDOM M1) UNIV` by METIS_TAC [bir_var_set_is_well_typed_INJ_DEF,
-  INJ_SUBSET, SUBSET_REFL, DIFF_SUBSET] >>
-
-`!v v'. v IN vs2 ==> (
-    ((bir_var_name v = bir_var_name v') /\ v' IN (vs2 DIFF vs1)) <=>
-    (~(v IN vs1) /\ (v' = v)))` by (
-
-  SIMP_TAC std_ss [IN_DIFF] >> REPEAT STRIP_TAC >>
-  METIS_TAC[bir_var_set_is_well_typed_def, SUBSET_DEF, bir_var_eq_EXPAND]
-) >>
-
-REPEAT STRIP_TAC >- (
-  SIMP_TAC std_ss [bir_env_EQ_FOR_VARS_def] >>
-  REPEAT STRIP_TAC >>
-  `v IN vs2` by METIS_TAC[SUBSET_DEF] >>
-  ASM_SIMP_TAC std_ss [bir_env_lookup_def, FLOOKUP_FUNION, FLOOKUP_MAP_KEYS]
-) >>
-
-FULL_SIMP_TAC std_ss [bir_env_vars_are_initialised_def]  >>
-Cases >> rename1 `BVar vn vty` >>
-STRIP_TAC >>
-REPEAT (Q.PAT_X_ASSUM `!v. _` (MP_TAC o Q.SPEC `BVar vn vty`)) >>
-FULL_SIMP_TAC std_ss [bir_env_var_is_initialised_def,
-  bir_env_lookup_def, FLOOKUP_MAP_KEYS,
-  FLOOKUP_FUNION, bir_var_name_def] >>
-Cases_on `BVar vn vty IN vs1` >- (
-  ASM_SIMP_TAC std_ss []
-) >>
-Q.UNABBREV_TAC `M1` >>
-Q.UNABBREV_TAC `VF` >>
-ASM_SIMP_TAC std_ss [FLOOKUP_FUN_FMAP, FINITE_DIFF,
-  bir_default_value_of_type_SPEC, bir_var_type_def, IN_DIFF]);
-
-
-
-val bir_env_vars_are_initialised_ENV_EXISTS_IFF = store_thm ("bir_env_vars_are_initialised_ENV_EXISTS_IFF",
-  ``!vs. (?env. bir_env_vars_are_initialised env vs) <=> (FINITE vs /\ bir_var_set_is_well_typed vs)``,
-
-GEN_TAC >> EQ_TAC >- (
-  METIS_TAC[bir_env_vars_are_initialised_WELL_TYPED, bir_env_vars_are_initialised_FINITE]
-) >>
-REPEAT STRIP_TAC >>
-MP_TAC (Q.SPECL [`{}`, `vs`, `bir_empty_env`] bir_env_vars_are_initialised_ENV_EXISTS_EXTENSION) >>
-ASM_SIMP_TAC std_ss [EMPTY_SUBSET, bir_env_vars_are_initialised_EMPTY, NOT_IN_EMPTY,
-  bir_env_EQ_FOR_VARS_EMPTY]);
-
-*)
 
 
 (* ===================== *)
